Dafny/AbstractNonInterferenceProof.s.dfy
@@ -1,0 +1,48 @@
+include "LLVM/llvm.i.dfy" // needs to be re-factored
+include "LLVM/control_flow.i.dfy"
+include "LLVM/types.dfy"
+include "LLVM/Operations/otherOperations.i.dfy"
+
+abstract module AbstractNonInterferenceProof {
+    import opened LLVM_def
+    import opened control_flow
+
+
+    predicate MiniSpec(s:LLVM_def.state, s':LLVM_def.state)
+
+    predicate ModuloMiniSpec(code:lvm_code, s:LLVM_def.state, s':LLVM_def.state,stateSeqS:seq<state>){
+        && startAndEndState(s,s',stateSeqS) 
+        && ValidStateSeq(stateSeqS) 
+        && StateSeqEvalsCode(code,stateSeqS)
+        && (forall i :: (i >=0 && i < |stateSeqS|-2) ==> !MiniSpec(stateSeqS[i],stateSeqS[i+1]))
+    }
+
+    lemma nonInterference(code:lvm_code, code':lvm_code,
+                          s:LLVM_def.state, s':LLVM_def.state, 
+                          r:LLVM_def.state, r':LLVM_def.state)
+        requires evalCode(code, s, s')
+        requires evalCode(code', r, r')
+        ensures forall stateSeqS:seq<state>, stateSeqR:seq<state> 
+                ::  (&& startAndEndState(s,s',stateSeqS) 
+                    && ValidStateSeq(stateSeqS) 
+                    && startAndEndState(r,r',stateSeqR) 
+                    && ValidStateSeq(stateSeqR)
+                    && ModuloMiniSpec(code,s,s',stateSeqS)) ==> lvm_state_eq(s',r')
+}
+
+
+
+/*
+    what is the MiniSpec?
+    MiniSpec is a single state predicate that describes incorrect behavior (that is supposedly fixed by the patch)
+
+        This would preclude all exections where there is a state that enters a 'danger' state. but not 
+        > necessarily 'act' on it
+
+    MiniSpec is a two-state predicate (s,s') that describes both the incorrect behavior and that incorrect behavior 
+    > dictates the state transition from s to s'
+        
+        This only reasons about the exections where a state s enters a 'danger' state *and* makes the 
+        > corresponding transition 
+*/
+    
