Dafny/LLVM/Operations/binaryOperations.i.dfy
@@ -22,8 +22,6 @@ module binary_operations_i {
         ensures typesMatch(v0,v1)
         ensures ToTwosComp(out).val == (v0.val + v1.val) % Pow256(v0.itype.size)
     { 
-        reveal_ToTwosComp();
-        reveal_FromTwosComp();
         if (v0.itype.size == 1) then evalADD8(size,v0,v1) else
         if (v0.itype.size == 2) then evalADD16(size,v0,v1) else
         if (v0.itype.size == 4) then evalADD32(size,v0,v1) else
@@ -45,8 +43,7 @@ module binary_operations_i {
         ensures ToTwosComp(out).val == (v0.val - v1.val) % Pow256(v0.itype.size)
 
     { 
-        reveal_ToTwosComp();
-        reveal_FromTwosComp();
+        
         if (v0.itype.size == 1) then evalSUB8(size,v0,v1) else
         if (v0.itype.size == 2) then evalSUB16(size,v0,v1) else
         if (v0.itype.size == 4) then evalSUB32(size,v0,v1) else
@@ -66,21 +63,21 @@ module binary_operations_i {
     lemma evalADD8check_unsigned()
     {
         reveal_BitwiseAdd8();
-        reveal_ToTwosComp();
+        
         assert forall d0,d1:Data :: isInt(d0) && isInt(d1) && typesMatch(d0,d1) && d0.itype == IntType(1, false) 
                                     ==> evalADD(1,d0,d1).val == (d0.val+d1.val) % Pow256(1);   
     }    
     lemma evalADD16check_unsigned()
     {
         reveal_BitwiseAdd16();
-        reveal_ToTwosComp();
+        
         assert forall d0,d1:Data :: isInt(d0) && isInt(d1) && typesMatch(d0,d1) && d0.itype == IntType(2, false) 
                                     ==> evalADD(2,d0,d1).val == (d0.val+d1.val) % Pow256(2);
     }
     lemma evalADD32check_unsigned()
     {
         reveal_BitwiseAdd32();
-        reveal_ToTwosComp();
+        
         assert forall d0,d1:Data :: isInt(d0) && isInt(d1) && typesMatch(d0,d1) && d0.itype == IntType(4, false) 
                                     ==> evalADD(4,d0,d1).val == (d0.val+d1.val) % Pow256(4);
     }
@@ -88,7 +85,7 @@ module binary_operations_i {
         lemma evalADD64check_unsigned()
     {
         reveal_BitwiseAdd64(); 
-        reveal_ToTwosComp();    
+            
         assert forall d0,d1:Data :: isInt(d0) && isInt(d1) && typesMatch(d0,d1) && d0.itype == IntType(8, false) 
                                     ==> evalADD(8,d0,d1).val == (d0.val+d1.val) % Pow256(8);
     }
@@ -96,8 +93,7 @@ module binary_operations_i {
     lemma evalADD8check_signed()
     {
         reveal_BitwiseAdd8();
-        reveal_ToTwosComp();
-        reveal_FromTwosComp();
+        
       
         assert forall d0,d1:Data :: isInt(d0) && isInt(d1) && typesMatch(d0,d1) && d0.itype == IntType(1, true) 
                                     ==> ToTwosComp(evalADD(1,d0,d1)).val == (d0.val+d1.val) % Pow256(1);   
@@ -105,8 +101,7 @@ module binary_operations_i {
     lemma evalADD16check_signed()
     {
         reveal_BitwiseAdd16();
-        reveal_ToTwosComp();
-        reveal_FromTwosComp();
+        
       
         assert forall d0,d1:Data :: isInt(d0) && isInt(d1) && typesMatch(d0,d1) && d0.itype == IntType(2, true) 
                                     ==> ToTwosComp(evalADD(2,d0,d1)).val == (d0.val+d1.val) % Pow256(2);    
@@ -114,8 +109,7 @@ module binary_operations_i {
     lemma evalADD32check_signed()
     {
         reveal_BitwiseAdd32();
-        reveal_ToTwosComp();
-        reveal_FromTwosComp();
+        
       
         assert forall d0,d1:Data :: isInt(d0) && isInt(d1) && typesMatch(d0,d1) && d0.itype == IntType(4, true) 
                                     ==> ToTwosComp(evalADD(4,d0,d1)).val == (d0.val+d1.val) % Pow256(4);    
@@ -123,8 +117,7 @@ module binary_operations_i {
     lemma evalADD64check_signed()
     {
         reveal_BitwiseAdd64();
-        reveal_ToTwosComp();
-        reveal_FromTwosComp();
+        
       
         assert forall d0,d1:Data :: isInt(d0) && isInt(d1) && typesMatch(d0,d1) && d0.itype == IntType(8, true) 
                                     ==> ToTwosComp(evalADD(8,d0,d1)).val == (d0.val+d1.val) % Pow256(8);   
@@ -134,28 +127,28 @@ module binary_operations_i {
 lemma evalSUB8check_unsigned()
     {
         reveal_BitwiseSub8();
-        reveal_ToTwosComp();
+        
         assert forall d0,d1:Data :: isInt(d0) && isInt(d1) && typesMatch(d0,d1) && d0.itype == IntType(1, false) 
                                     ==> evalSUB(1,d0,d1).val == (d0.val-d1.val) % Pow256(1);   
     }
 lemma evalSUB16check_unsigned()
     {
         reveal_BitwiseSub16();
-        reveal_ToTwosComp();
+        
         assert forall d0,d1:Data :: isInt(d0) && isInt(d1) && typesMatch(d0,d1) && d0.itype == IntType(2, false) 
                                     ==> evalSUB(2,d0,d1).val == (d0.val-d1.val) % Pow256(2);   
     }
 lemma evalSUB32check_unsigned()
     {
         reveal_BitwiseSub32();
-        reveal_ToTwosComp();
+        
         assert forall d0,d1:Data :: isInt(d0) && isInt(d1) && typesMatch(d0,d1) && d0.itype == IntType(4, false) 
                                     ==> evalSUB(4,d0,d1).val == (d0.val-d1.val) % Pow256(4);   
     }
 lemma evalSUB64check_unsigned()
     {
         reveal_BitwiseSub64();
-        reveal_ToTwosComp();
+        
         assert forall d0,d1:Data :: isInt(d0) && isInt(d1) && typesMatch(d0,d1) && d0.itype == IntType(8, false) 
                                     ==> evalSUB(8,d0,d1).val == (d0.val-d1.val) % Pow256(8);   
     }
@@ -163,28 +156,28 @@ lemma evalSUB64check_unsigned()
 lemma evalSUB8check_signed()
     {
         reveal_BitwiseSub8();
-        reveal_ToTwosComp();
+        
         assert forall d0,d1:Data :: isInt(d0) && isInt(d1) && typesMatch(d0,d1) && d0.itype == IntType(1, false) 
                                     ==> ToTwosComp(evalSUB(1,d0,d1)).val == (d0.val-d1.val) % Pow256(1);   
     }
 lemma evalSUB16check_signed()
     {
         reveal_BitwiseSub16();
-        reveal_ToTwosComp();
+        
         assert forall d0,d1:Data :: isInt(d0) && isInt(d1) && typesMatch(d0,d1) && d0.itype == IntType(2, false) 
                                     ==> ToTwosComp(evalSUB(2,d0,d1)).val == (d0.val-d1.val) % Pow256(2);   
     }
 lemma evalSUB32check_signed()
     {
         reveal_BitwiseSub32();
-        reveal_ToTwosComp();
+        
         assert forall d0,d1:Data :: isInt(d0) && isInt(d1) && typesMatch(d0,d1) && d0.itype == IntType(4, false) 
                                     ==> ToTwosComp(evalSUB(4,d0,d1)).val == (d0.val-d1.val) % Pow256(4);   
     }
 lemma evalSUB64check_signed()
     {
         reveal_BitwiseSub64();
-        reveal_ToTwosComp();
+        
         assert forall d0,d1:Data :: isInt(d0) && isInt(d1) && typesMatch(d0,d1) && d0.itype == IntType(8, false) 
                                     ==> ToTwosComp(evalSUB(8,d0,d1)).val == (d0.val-d1.val) % Pow256(8);   
     }
