Dafny/NonInterferenceTest.i.dfy
@@ -1,0 +1,76 @@
+//// TEST EXAMPLES
+include "./AbstractNonInterferenceProof.s.dfy" 
+include "LLVM/control_flow.i.dfy"
+include "LLVM/types.dfy"
+
+module challenge5 refines AbstractNonInterferenceProof {
+    import opened types
+    import opened other_operations_i
+    
+    
+     function {:opaque} encrypt(plainText:Data):codes
+    {
+        ForeignFunction
+    }
+
+    predicate MiniSpec(s:LLVM_def.state, s':LLVM_def.state)
+    {
+        reveal_encrypt();
+
+        && StateNext(s,s') 
+        && forall plainText :: evalBlock(encrypt(plainText),s,s') ==> s == s'
+    }
+    
+
+        
+    predicate MiniSpecCH_P1Single(s:LLVM_def.state)
+    {
+        && ValidState(s) 
+        && (exists speed_value:operand ::
+            (   && speed_value.LV?
+                && ValidOperand(s,speed_value)
+                && OperandContents(s,speed_value).Int?
+                && typesMatch(OperandContents(s,speed_value),Int(0,IntType(2,false)))
+                && OperandContents(s,speed_value).val > 0 
+                && evalICMP(sgt,2,OperandContents(s,speed_value),Int(0,IntType(2,false))).val == 0))
+
+    }
+
+    predicate ModuloMiniCH_P1Single(code:lvm_code, stateSeq:seq<state>)
+    {
+        && StateSeqEvalsCode(code,stateSeq)
+        && (forall i :: (i >=0 && i <|stateSeq|) ==> !MiniSpecCH_P1Single(stateSeq[i]))
+    }
+
+
+    predicate MiniSpecCH_P1Double(s:LLVM_def.state, s':LLVM_def.state)
+    {
+        && MiniSpecCH_P1Single(s)
+        && StateNext(s,s') 
+        && s != s'
+        && exists cmp:ins :: (cmp.ICMP? && ValidInstruction(s,cmp) && evalIns(cmp, s, s'))
+    }
+
+    predicate ModuloMiniCH_P1Double(code:lvm_code, stateSeq:seq<state>)
+    {
+        && StateSeqEvalsCode(code,stateSeq)
+        && (forall i :: (i >=0 && i <|stateSeq|-2) ==> !MiniSpecCH_P1Double(stateSeq[i],stateSeq[i+1]))
+    }
+
+
+    lemma nonInterferenceCH_P1Single(code:lvm_code, code':lvm_code,
+                          s:LLVM_def.state, s':LLVM_def.state, 
+                          r:LLVM_def.state, r':LLVM_def.state)
+        requires evalCode(code, s, s')
+        requires evalCode(code', r, r')
+        ensures forall stateSeqS:seq<state>, stateSeqR:seq<state> 
+                ::  (&& startAndEndState(s,s',stateSeqS) 
+                    && ValidStateSeq(stateSeqS) 
+                    && startAndEndState(r,r',stateSeqR) 
+                    && ValidStateSeq(stateSeqR)
+                    && ModuloMiniCH_P1Double(code,stateSeqS)) ==> lvm_state_eq(s',r') //might need to compare full seq?   
+                    // {
+
+                    // }
+
+}
