SConstruct
@@ -324,12 +324,10 @@ def run_directory(dir_name, dafny_files):
 
 if verify_root is None:
   print("==> No .dfy root specified, verifying all .dfy files in Dafny/examples folder")
-  run_directory('Dafny/examples',["challengeProblem1Simplified",
-                                      "simple",
-                                      "demoChallengeProb1",
-                                      "demoChallengeProb1VulnNoAssert",
-                                      "musings",
-                                      "Challenge4"])
+  run_directory('Dafny/examples',["simple",
+                                  "demoChallengeProb1",
+                                  "demoChallengeProb1VulnNoAssert",
+                                  "Challenge4"])
 else:
   verify_dafny_file(str(GetOption('verify_root')))
 
